docs/research/2026-09-02-shared-semantics/rows/explicit_16.lean
@@ -1,0 +1,16 @@
+import Effects.Morphism
+set_option warn.classDefReducibility false
+open Effects
+universe uS uR uL uA
+class Has (S : Signature.{uS,uA}) (R : Signature.{uR,uA}) where
+  hom : Signature.Hom S R
+instance (priority := 1000) : Has S S := ⟨Signature.Hom.id S⟩
+instance (priority := 900) : Has S (S ⊕ₛ T) := ⟨Signature.Hom.inl⟩
+instance (priority := 800) [h : Has S R] : Has S (L ⊕ₛ R) :=
+  ⟨h.hom.comp Signature.Hom.inr⟩
+inductive Tag (n : Nat) where | tag
+def atom (n : Nat) : Signature := ⟨Tag n, fun _ => Unit⟩
+abbrev row : Signature := (atom 0 ⊕ₛ (atom 1 ⊕ₛ (atom 2 ⊕ₛ (atom 3 ⊕ₛ (atom 4 ⊕ₛ (atom 5 ⊕ₛ (atom 6 ⊕ₛ (atom 7 ⊕ₛ (atom 8 ⊕ₛ (atom 9 ⊕ₛ (atom 10 ⊕ₛ (atom 11 ⊕ₛ (atom 12 ⊕ₛ (atom 13 ⊕ₛ (atom 14 ⊕ₛ atom 15)))))))))))))))
+def witness0 : Signature.Hom (atom 0) row := Signature.Hom.inl
+def witness8 : Signature.Hom (atom 8) row := ((((((((Signature.Hom.inl).comp Signature.Hom.inr).comp Signature.Hom.inr).comp Signature.Hom.inr).comp Signature.Hom.inr).comp Signature.Hom.inr).comp Signature.Hom.inr).comp Signature.Hom.inr).comp Signature.Hom.inr
+def witness15 : Signature.Hom (atom 15) row := (((((((((((((((Signature.Hom.id _).comp Signature.Hom.inr).comp Signature.Hom.inr).comp Signature.Hom.inr).comp Signature.Hom.inr).comp Signature.Hom.inr).comp Signature.Hom.inr).comp Signature.Hom.inr).comp Signature.Hom.inr).comp Signature.Hom.inr).comp Signature.Hom.inr).comp Signature.Hom.inr).comp Signature.Hom.inr).comp Signature.Hom.inr).comp Signature.Hom.inr).comp Signature.Hom.inr
