docs/research/2026-09-02-shared-semantics/rows/missing_member.lean
@@ -1,0 +1,14 @@
+import Effects.Morphism
+set_option warn.classDefReducibility false
+open Effects
+universe uS uR uL uA
+class Has (S : Signature.{uS,uA}) (R : Signature.{uR,uA}) where
+  hom : Signature.Hom S R
+instance (priority := 1000) : Has S S := ⟨Signature.Hom.id S⟩
+instance (priority := 900) : Has S (S ⊕ₛ T) := ⟨Signature.Hom.inl⟩
+instance (priority := 800) [h : Has S R] : Has S (L ⊕ₛ R) :=
+  ⟨h.hom.comp Signature.Hom.inr⟩
+inductive Tag (n : Nat) where | tag
+def atom (n : Nat) : Signature := ⟨Tag n, fun _ => Unit⟩
+abbrev row : Signature := atom 0 ⊕ₛ atom 1
+def witness : Has (atom 2) row := inferInstance
